checkpoint trace-based plan

src/Spec/Trace.v
@@ -2,6 +2,7 @@ Require Import Relations.Relation_Operators.
 Require Import RelationClasses.
 Require Import ClassicalFacts.
 Require Import FunctionalExtensionality.
+Require Import Omega.
 Require Import Helpers.Helpers.
 
 Axiom EM : excluded_middle.
@@ -89,7 +90,8 @@ Inductive opT : Type -> Type :=
 | Inc : opT nat.
 
 Inductive opHiT : Type -> Type :=
-| IncTwice : opHiT nat.
+| IncTwice : opHiT nat
+| Noop : opHiT unit.
 
 Inductive opHi2T : Type -> Type :=
 .
@@ -102,18 +104,26 @@ Inductive op_step : forall T, opT T -> nat -> State -> T -> State -> Prop :=
 
 Inductive opHi_step : forall T, opHiT T -> nat -> State -> T -> State -> Prop :=
 | StepIncTwice : forall tid n,
-  opHi_step IncTwice tid n (n+2) (n+2).
+  opHi_step IncTwice tid n (n+2) (n+2)
+| StepNoop : forall tid n,
+  opHi_step Noop tid n tt n.
 
 
 Definition threads_empty {opT opHiT} : threads_state opT opHiT :=
   fun x => None.
 
-Definition ts := thread_upd threads_empty 1
+Definition inc_twice_impl :=
   (Bind (InvokeOpHi opT opHiT _ IncTwice) (fun _ =>
   (Bind (Op opT opHiT _ Inc) (fun i1 =>
   (Bind (Op opT opHiT _ Inc) (fun i2 =>
   (Bind (ReturnOpHi opT opHiT i2) (fun _ =>
-        (Ret opT opHiT tt))))))))).
+        (Ret opT opHiT i2))))))))).
+
+Definition p1 :=
+  (Bind inc_twice_impl (fun _ =>
+        (Ret opT opHiT tt))).
+
+Definition ts := thread_upd threads_empty 1 p1.
 
 Lemma thread_upd_eq : forall opT opHiT ts p tid,
   @thread_upd opT opHiT ts tid p tid = Some p.
@@ -145,21 +155,41 @@ Definition ex_trace :
   { t : trace opT opHiT | exec op_step 4 ts t }.
 Proof.
   eexists.
+  eapply ExecBind with (tid := 1).
+    unfold ts.
+    rewrite thread_upd_eq.
+    reflexivity.
   eapply ExecInvokeHi with (tid := 1).
     unfold ts.
     rewrite thread_upd_eq.
     reflexivity.
+  eapply ExecBind with (tid := 1).
+    unfold ts.
+    rewrite thread_upd_eq.
+    reflexivity.
   eapply ExecOp with (tid := 1).
     unfold ts.
     rewrite thread_upd_eq.
     reflexivity.
     constructor.
+  eapply ExecBind with (tid := 1).
+    unfold ts.
+    rewrite thread_upd_eq.
+    reflexivity.
   eapply ExecOp with (tid := 1).
     unfold ts.
     rewrite thread_upd_eq.
     reflexivity.
     constructor.
+  eapply ExecBind with (tid := 1).
+    unfold ts.
+    rewrite thread_upd_eq.
+    reflexivity.
   eapply ExecReturnHi with (tid := 1).
+    unfold ts.
+    rewrite thread_upd_eq.
+    reflexivity.
+  eapply ExecRet with (tid := 1).
     unfold ts.
     rewrite thread_upd_eq.
     reflexivity.
@@ -176,9 +206,11 @@ Defined.
 Eval compute in (proj1_sig ex_trace).
 
 
-Definition ts2 := thread_upd threads_empty 1
+Definition p2 :=
   (Bind (Op opHiT opHi2T _ IncTwice) (fun _ =>
         (Ret opHiT opHi2T tt))).
+
+Definition ts2 := thread_upd threads_empty 1 p2.
 
 Definition ex_trace2 :
   { t : trace opHiT opHi2T | exec opHi_step 4 ts2 t }.
@@ -242,4 +274,210 @@ Theorem ex_trace_ex_trace2 :
 Proof.
   simpl.
   eauto 10.
+Qed.
+
+
+Inductive compile_ok : forall T (p1 : proc opT opHiT T) (p2 : proc opHiT opHi2T T), Prop :=
+| CompileIncTwice :
+  compile_ok (inc_twice_impl) (Op opHiT opHi2T _ IncTwice)
+| CompileRet : forall T (x : T),
+  compile_ok (Ret opT opHiT x) (Ret opHiT opHi2T x)
+| CompileBind : forall T1 T2 (p1a : proc opT opHiT T1) (p2a : proc opHiT opHi2T T1)
+                             (p1b : T1 -> proc opT opHiT T2) (p2b : T1 -> proc opHiT opHi2T T2),
+  compile_ok p1a p2a ->
+  (forall x, compile_ok (p1b x) (p2b x)) ->
+  compile_ok (Bind p1a p1b) (Bind p2a p2b).
+
+Theorem ex_compile_ok : compile_ok p1 p2.
+Proof.
+  unfold p1, p2.
+  econstructor.
+  econstructor.
+  intros. econstructor.
+Qed.
+
+Hint Resolve ex_compile_ok.
+
+Definition threads_compile_ok (ts1 : threads_state opT opHiT) (ts2 : threads_state opHiT opHi2T) :=
+  forall tid,
+    ts1 tid = None /\ ts2 tid = None \/
+  (exists p1 p2,
+    ts1 tid = Some p1 /\ ts2 tid = Some p2 /\ compile_ok p1 p2).
+
+Theorem ex_ts_compile_ok : threads_compile_ok ts ts2.
+Proof.
+  unfold threads_compile_ok, ts, ts2, thread_upd, threads_empty; intros.
+  destruct (1 == tid); intuition eauto.
+Qed.
+
+Lemma thread_upd_inv : forall opT opHiT ts tid1 p tid2 p',
+  @thread_upd opT opHiT ts tid1 p tid2 = Some p' ->
+  tid1 = tid2 /\ p = p' \/
+  tid1 <> tid2 /\ ts tid2 = Some p'.
+Proof.
+  unfold thread_upd; intros.
+  destruct (tid1 == tid2); intuition eauto.
+  inversion H; eauto.
+Qed.
+
+Lemma thread_empty_inv : forall opT opHiT tid p',
+  @threads_empty opT opHiT tid = Some p' ->
+  False.
+Proof.
+  unfold threads_empty; intros; congruence.
+Qed.
+
+Lemma thread_upd_not_empty : forall opT opHiT tid ts p,
+  (forall tid', @thread_upd opT opHiT ts tid p tid' = None) -> False.
+Proof.
+  unfold thread_upd; intros.
+  specialize (H tid).
+  destruct (tid == tid); congruence.
+Qed.
+
+Lemma thread_upd_upd_eq : forall opT opHiT ts tid p1 p2,
+  @thread_upd opT opHiT (thread_upd ts tid p1) tid p2 =
+  thread_upd ts tid p2.
+Proof.
+  unfold thread_upd; intros.
+  apply functional_extensionality; intros.
+  destruct (tid == x); congruence.
+Qed.
+
+
+Ltac thread_inv :=
+  match goal with
+  | H : thread_upd _ _ _ _ = Some _ |- _ =>
+    eapply thread_upd_inv in H; destruct H; (intuition idtac); subst
+  | H : threads_empty _ = Some _ |- _ =>
+    eapply thread_empty_inv in H; exfalso; apply H
+  | H : _ = Bind _ _ |- _ =>
+    solve [ inversion H ]
+  | H : _ = Ret _ _ _|- _ =>
+    solve [ inversion H ]
+  | H : forall _, thread_upd _ _ _ _ = None |- _ =>
+    solve [ eapply thread_upd_not_empty in H; exfalso; eauto ]
+  end.
+
+Ltac bind_inv :=
+  match goal with
+  | H : _ = Bind _ _ |- _ =>
+    inversion H; clear H; subst; repeat sigT_eq
+  end.
+
+Ltac exec_inv :=
+  match goal with
+  | H : exec _ _ _ _ |- _ =>
+    inversion H; clear H; subst
+  end;
+  autorewrite with t in *.
+
+
+Hint Rewrite thread_upd_upd_eq : t.
+Hint Rewrite thread_del_upd_eq : t.
+Hint Rewrite thread_del_empty : t.
+
+Ltac empty_inv :=
+  try solve [ exfalso; eapply thread_empty_inv; eauto ].
+
+Ltac step_inv :=
+  match goal with
+  | H : op_step _ _ _ _ _ |- _ =>
+    inversion H; clear H; subst; repeat sigT_eq
+  | H : opHi_step _ _ _ _ _ |- _ =>
+    inversion H; clear H; subst; repeat sigT_eq
+  end.
+
+Theorem ex_all_traces_match :
+  forall s tr1 tr2,
+  exec op_step s ts tr1 ->
+  exec opHi_step s ts2 tr2 ->
+  traces_match tr1 tr2.
+Proof.
+  intros.
+  unfold ts, ts2 in *.
+
+  exec_inv; repeat thread_inv; bind_inv.
+  exec_inv; repeat thread_inv.
+  exec_inv; repeat thread_inv; empty_inv.
+
+  exec_inv; repeat thread_inv; bind_inv.
+  exec_inv; repeat thread_inv; bind_inv.
+  exec_inv; repeat thread_inv; bind_inv.
+  exec_inv; repeat thread_inv; bind_inv.
+  exec_inv; repeat thread_inv; bind_inv.
+  exec_inv; repeat thread_inv; bind_inv.
+  exec_inv; repeat thread_inv; bind_inv.
+  exec_inv; repeat thread_inv; bind_inv.
+  exec_inv; repeat thread_inv; bind_inv.
+  exec_inv; repeat thread_inv.
+  exec_inv; repeat thread_inv; empty_inv.
+
+  step_inv.
+  step_inv.
+  step_inv.
+
+  replace (s + 1 + 1) with (s + 2) by omega.
+  eauto 20.
+Qed.
+
+
+Lemma helper1 : forall S opT opHiT step (s : S) tid p (tr : trace opT opHiT),
+  exec step s (thread_upd threads_empty tid p) tr ->
+  exec step s (thread_upd threads_empty tid (Bind p (fun _ => Ret _ _ tt))) tr.
+Proof.
+Admitted.
+
+
+(**
+ PLAN:
+ two proof styles:
+  - state correspondence like in POCS
+  - commute operations in low level while preserving high-level trace
+ The theorem below tries to do state correspondence, in a way.
+
+ Need to figure out how to deal with semicolon.
+ Need to figure out how to generalize the [compile_ok p1 p2] statement to
+  allow for some partially-executed code inside of [p1].  This corresponds
+  to some relation between states [s2] and [s1] in the high and low levels,
+  respectively.
+*)
+
+(**
+ TODO: introduce notion of atomicity.
+
+ In particular, we would like to show that the low-level implementation opcodes
+ (i.e., Inc) can be commuted to produce atomic groups of more than one opcode.
+ Then, we can group the entire inc_twice_impl into a single atomic unit.  Then
+ this might simplify our proof.
+*)
+
+Theorem all_single_thread_traces_match' :
+  forall s tr1 tr2 T (p1 : proc opT opHiT T) (p2 : proc opHiT opHi2T T),
+  compile_ok p1 p2 ->
+  exec op_step s (thread_upd threads_empty 1 (Bind p1 (fun _ => Ret _ _ tt))) tr1 ->
+  exec opHi_step s (thread_upd threads_empty 1 (Bind p2 (fun _ => Ret _ _ tt))) tr2 ->
+  traces_match tr1 tr2.
+Proof.
+  intros.
+  generalize dependent tr1.
+  generalize dependent tr2.
+  induction H; intros.
+  - admit.
+  - admit.
+  - 
+
+Admitted.
+
+Theorem all_single_thread_traces_match :
+  forall s tr1 tr2 p1 p2,
+  compile_ok p1 p2 ->
+  exec op_step s (thread_upd threads_empty 1 p1) tr1 ->
+  exec opHi_step s (thread_upd threads_empty 1 p2) tr2 ->
+  traces_match tr1 tr2.
+Proof.
+  intros.
+  eapply all_single_thread_traces_match'; eauto.
+  eapply helper1; eauto.
+  eapply helper1; eauto.
 Qed.
